HL.lean
@@ -3,6 +3,7 @@ import SFLMeta.Ignore
 import SFLMeta.Save
 
 import HL.Intro
+import HL.Imp
 
 import VersoManual
 
@@ -10,3 +11,4 @@ open Verso Genre Manual
 
 #doc (Manual) "Hoare Logic" =>
 {include HL.Intro}
+{include HL.Imp}
